nola/iris/sinv.v
@@ -42,16 +42,16 @@ Section sinv.
   Local Definition sinv_auth_tok M :=
     own sinv_name (gmap_view_auth (DfracOwn 1) (to_agree <$> M)).
   (** World satisfaction *)
-  Definition sinv_iwsat_def ip : iProp Σ :=
-    ∃ M, sinv_auth_tok M ∗ [∗ map] i ↦ P ∈ M, ip i P.
+  Definition sinv_iwsat_def sm : iProp Σ :=
+    ∃ M, sinv_auth_tok M ∗ [∗ map] i ↦ P ∈ M, sm i P.
   Local Lemma sinv_iwsat_aux : seal sinv_iwsat_def. Proof. by eexists. Qed.
   Definition sinv_iwsat := sinv_iwsat_aux.(unseal).
   Local Lemma sinv_iwsat_unseal : sinv_iwsat = sinv_iwsat_def.
   Proof. exact: seal_eq. Qed.
 End sinv.
-(** World satisfaction whose interpretation ignores the index *)
-Notation sinv_wsat' FML ip := (sinv_iwsat (FML:=FML) (λ _, ip)).
-Notation sinv_wsat ip := (sinv_wsat' _ ip).
+(** World satisfaction whose semantics ignores the index *)
+Notation sinv_wsat' FML sm := (sinv_iwsat (FML:=FML) (λ _, sm)).
+Notation sinv_wsat sm := (sinv_wsat' _ sm).
 
 Section sinv.
   Context `{!sinvGS FML Σ}.
@@ -84,11 +84,11 @@ Section sinv.
     Proper (pointwise_relation _ (pointwise_relation _ (≡)) ==> (≡)) sinv_iwsat.
   Proof. rewrite sinv_iwsat_unseal. solve_proper. Qed.
 
-  (** [sinv_iwsat] is timeless if [ip] is always timeless
+  (** [sinv_iwsat] is timeless if [sm] is always timeless
     and the underlying ofe is discrete *)
   #[export] Instance sinv_iwsat_timeless
-    `{!OfeDiscrete (FML $oi Σ), !∀ i P, Timeless (ip i P)} :
-    Timeless (sinv_iwsat ip).
+    `{!OfeDiscrete (FML $oi Σ), !∀ i P, Timeless (sm i P)} :
+    Timeless (sinv_iwsat sm).
   Proof. rewrite sinv_iwsat_unseal. exact _. Qed.
 
   (** Lemma for [sinv_itok_alloc] *)
@@ -100,17 +100,17 @@ Section sinv.
     apply gmap_view_alloc; [|done..]. by rewrite lookup_fmap eq.
   Qed.
   (** Allocate [sinv_itok] *)
-  Lemma sinv_itok_alloc {ip} P :
-    sinv_iwsat ip -∗ ∃ I, ∀ i, ⌜i ∉ I⌝ ==∗
-      sinv_itok i P ∗ (ip i P -∗ sinv_iwsat ip).
+  Lemma sinv_itok_alloc {sm} P :
+    sinv_iwsat sm -∗ ∃ I, ∀ i, ⌜i ∉ I⌝ ==∗
+      sinv_itok i P ∗ (sm i P -∗ sinv_iwsat sm).
   Proof.
     rewrite sinv_iwsat_unseal. iIntros "[%M[● M]]". iExists (dom M).
     iIntros (i ?). iMod (sinv_auth_tok_alloc with "●") as "[● #i]"; [done|].
     iModIntro. iSplitR; [by rewrite sinv_itok_unseal|]. iIntros "P". iExists _.
     iFrame "●". iApply (big_sepM_insert_2 with "P M").
   Qed.
-  Lemma sinv_tok_alloc {ip} P :
-    sinv_wsat ip ==∗ sinv_tok P ∗ (ip P -∗ sinv_wsat ip).
+  Lemma sinv_tok_alloc {sm} P :
+    sinv_wsat sm ==∗ sinv_tok P ∗ (sm P -∗ sinv_wsat sm).
   Proof.
     iIntros "W". iDestruct (sinv_itok_alloc with "W") as (?) "big".
     iMod ("big" with "[]") as "[? $]". { iPureIntro. apply is_fresh. }
@@ -128,8 +128,8 @@ Section sinv.
     iExists P'. iSplit; [done|]. by rewrite to_agree_includedI.
   Qed.
   (** Access via [sinv_tok] *)
-  Lemma sinv_tok_acc' `{!NonExpansive (ip i)} {P} :
-    sinv_itok i P -∗ sinv_iwsat ip -∗ ip i P ∗ (ip i P -∗ sinv_iwsat ip).
+  Lemma sinv_tok_acc' `{!NonExpansive (sm i)} {P} :
+    sinv_itok i P -∗ sinv_iwsat sm -∗ sm i P ∗ (sm i P -∗ sinv_iwsat sm).
   Proof.
     rewrite sinv_iwsat_unseal. iIntros "i [%M[● M]]".
     iDestruct (sinv_auth_tok_lookup with "● i") as (P' eq) "#≡".
@@ -137,8 +137,8 @@ Section sinv.
     iRewrite "≡". iFrame "P'". iIntros "P'". iExists _. iFrame "●".
     by iApply "→M".
   Qed.
-  Lemma sinv_tok_acc `{!NonExpansive ip} {P} :
-    sinv_tok P -∗ sinv_wsat ip -∗ ip P ∗ (ip P -∗ sinv_wsat ip).
+  Lemma sinv_tok_acc `{!NonExpansive sm} {P} :
+    sinv_tok P -∗ sinv_wsat sm -∗ sm P ∗ (sm P -∗ sinv_wsat sm).
   Proof. iIntros "[%i i]". iApply (sinv_tok_acc' with "i"). Qed.
 End sinv.
 
@@ -151,7 +151,7 @@ Proof.
 Qed.
 (** Allocate [sinv_wsat] *)
 Lemma sinv_wsat_alloc `{!sinvGpreS FML Σ} :
-  ⊢ |==> ∃ _ : sinvGS FML Σ, ∀ ip, sinv_iwsat ip.
+  ⊢ |==> ∃ _ : sinvGS FML Σ, ∀ sm, sinv_iwsat sm.
 Proof.
   iMod sinv_auth_tok_alloc_empty as (?) "●". iModIntro. iExists _.
   iIntros. rewrite sinv_iwsat_unseal. iExists ∅. by iFrame.
