nola/util/sem.v
@@ -1,0 +1,23 @@
+(** * Semantics *)
+
+From nola Require Export prelude.
+
+(** ** [Sem]: Semantics *)
+Class Sem (A B : Type) := sem : A → B.
+Hint Mode Sem ! - : typeclass_instances.
+Module SemNotation.
+  Notation "⟦ ⟧" := (sem) (format "⟦ ⟧").
+  Notation "⟦ ⟧@{ A }" := (sem (A:=A)) (only parsing).
+  Notation "⟦ a ⟧" := (sem a) (format "⟦  '[' a  ']' ⟧").
+  Notation "⟦ a ⟧@{ A }" := (sem (A:=A) a) (only parsing).
+End SemNotation.
+
+(** ** [Psem]: Parameterized semantics *)
+Class Psem (X A B : Type) := psem : X → A → B.
+Hint Mode Psem - ! - : typeclass_instances.
+Module PsemNotation.
+  Notation "⟦ ⟧( x )" := (psem x) (format "⟦ ⟧( x )").
+  Notation "⟦ ⟧( x )@{ A }" := (psem (A:=A) x) (only parsing).
+  Notation "⟦ a ⟧( x )" := (psem x a) (format "⟦  '[' a  ']' ⟧( x )").
+  Notation "⟦ a ⟧( x )@{ A }" := (psem (A:=A) x a) (only parsing).
+End PsemNotation.
